frontend/Types.v
@@ -8,22 +8,25 @@
 Require Import Le.
 Require Import List.
 
+Require Import DecEqFacts.
 Require Import Symbol.
 
 Module Type UNIQUE.
 
   Parameter t : Set.
 
+  Parameter init : list t.
   Parameter new : list t -> list t * t.
-  Parameter dec : forall (u1 u2 : t), {u1 = u2} + {u1 <> u2}.
+  Parameter eq : forall (u1 u2 : t), {u1 = u2} + {u1 <> u2}.
 
   Definition is_unique (us : list t) : Prop := NoDup us.
 
-  Axiom new_adds : forall u us us',
-    new us = (us', u) ->
-    In u us'.
+  Hypothesis init_unique : is_unique init.
 
-  Axiom new_unique : forall us, is_unique us -> is_unique (fst (new us)).
+  Hypothesis new_spec : forall u us us',
+    is_unique us ->
+    new us = (us', u) ->
+    In u us' /\ is_unique us'.
 
 End UNIQUE.
 
@@ -33,11 +36,13 @@ Module Unique <: UNIQUE.
 
   Definition maximum (us : list t) := fold_right max 0 us.
 
+  Definition init := @nil t.
+
   Definition new (us : list t) :=
     let u := S (maximum us) in
     (u :: us, u).
 
-  Definition dec : forall (u1 u2 : t), {u1 = u2} + {u1 <> u2}.
+  Definition eq : forall (u1 u2 : t), {u1 = u2} + {u1 <> u2}.
     decide equality.
   Defined.
 
@@ -61,35 +66,30 @@ Module Unique <: UNIQUE.
   Lemma init_unique : is_unique nil.
   Proof. constructor. Qed.
 
-  Lemma new_adds : forall u us us',
+  Lemma new_spec : forall u us us',
+    is_unique us ->
     new us = (us', u) ->
-    In u us'.
+    In u us' /\ is_unique us'.
   Proof.
-    unfold new. intros.
-    inversion H; subst; constructor; reflexivity.
-  Qed.
-
-  Lemma new_unique : forall us, is_unique us -> is_unique (fst (new us)).
-  Proof.
-    unfold is_unique, new. intros.
-    induction us; simpl.
-    - constructor; auto.
-    - constructor; [| assumption].
-      change (max a (maximum us)) with (maximum (a :: us)).
-      unfold not. intros.
-      apply maximum_ge in H0.
-      apply Le.le_Sn_n in H0; assumption.
+    unfold new, is_unique; intros.
+    inversion H0; subst.
+    split.
+    - simpl; left; reflexivity.
+    - destruct us.
+      + constructor; auto.
+      + constructor; [| assumption].
+        unfold not; intros.
+        apply maximum_ge in H1.
+        apply Le.le_Sn_n in H1; assumption.
   Qed.
 
 End Unique.
 
-Module Types' (U : UNIQUE).
-
-  Definition symbol := Symbol.t.
+Module Types' (S : SYMBOL) (U : UNIQUE).
 
   Definition upool := list U.t.
 
-  Definition uinit : upool := nil.
+  Definition uinit : upool := U.init.
   Definition unew us : upool * U.t := U.new us.
 
   Inductive ty : Set :=
@@ -98,94 +98,50 @@ Module Types' (U : UNIQUE).
     | INT : ty
     | STRING : ty
     | ARRAY : ty -> U.t -> ty
-    | NAME : symbol -> ty
+    | NAME : S.t -> ty
     | UNIT : ty
   with rfield : Set :=
-    | mk_rfield : symbol -> ty -> rfield.
+    | mk_rfield : S.t -> ty -> rfield.
 
   Definition rf_name (rf : rfield) := let (name, _) := rf in name.
   Definition rf_type (rf : rfield) := let (_, type) := rf in type.
 
-  Fixpoint ty_dec (t1 t2 : ty) : {t1 = t2} + {t1 <> t2}.
-    repeat decide equality; try (apply U.dec).
+  Fixpoint ty_eq (t1 t2 : ty) : {t1 = t2} + {t1 <> t2}.
+    repeat decide equality; try apply U.eq; try apply S.eq.
   Defined.
 
-  Definition rf_eq (rf1 rf2 : rfield) : bool :=
-    if Symbol.eq (rf_name rf1) (rf_name rf2)
-      then if ty_dec (rf_type rf1) (rf_type rf2)
-        then true
-        else false
-      else false.
-
-  Lemma rf_eq_refl : forall rf,
-    rf_eq rf rf = true.
-  Proof.
-    intros; unfold rf_eq; rewrite Symbol.eq_refl.
-    destruct (ty_dec (rf_type rf) (rf_type rf)); congruence.
-  Qed.
-
-  Lemma rf_eq_sym : forall rf1 rf2,
-    rf_eq rf1 rf2 = rf_eq rf2 rf1.
-  Proof.
-    destruct rf1, rf2; unfold rf_eq;
-    simpl; rewrite Symbol.eq_sym.
-    destruct (Symbol.eq s0 s);
-    destruct (ty_dec t t0);
-    destruct (ty_dec t0 t);
-    try subst; congruence.
-  Qed.
-
-  Lemma rf_eq_trans : forall rf1 rf2 rf3,
-    rf_eq rf1 rf2 = true ->
-    rf_eq rf2 rf3 = true ->
-    rf_eq rf1 rf3 = true.
-  Proof.
-    unfold rf_eq; intros.
-    destruct (Symbol.eq (rf_name rf1) (rf_name rf2)) eqn:EQ1;
-    destruct (Symbol.eq (rf_name rf2) (rf_name rf3)) eqn:EQ2;
-    destruct (Symbol.eq (rf_name rf1) (rf_name rf3)) eqn:EQ3;
-    try (repeat match goal with
-    | [ H : (if ?X then _ else _) = _ |- _ ] => destruct X
-    | [ |- (if ?X then _ else _) = _ ] => destruct X
-    end; congruence).
-    generalize Symbol.eq_trans; intros.
-    specialize H1 with (rf_name rf1) (rf_name rf2) (rf_name rf3).
-    apply H1 in EQ1. congruence.
-    assumption.
-  Qed.
+  Definition rf_eq (rf1 rf2 : rfield) : {rf1 = rf2} + {rf1 <> rf2}.
+    decide equality; try apply ty_eq; try apply S.eq.
+  Defined.
 
   Definition ty_compat (t1 t2 : ty) : bool :=
-    if ty_dec t1 t2 then true
-    else match t1, t2 with
-    | RECORD _ u1, RECORD _ u2 => if U.dec u1 u2 then true else false
-    | RECORD fs u, NIL => true
-    | NIL, RECORD fs u => true
+    if ty_eq t1 t2
+      then true
+      else match t1, t2 with
+      | RECORD _ u1, RECORD _ u2 => if U.eq u1 u2 then true else false
+      | RECORD fs u, NIL => true
+      | NIL, RECORD fs u => true
+      | _, _ => false
+      end.
+
+  Fixpoint tys_compat (ts1 ts2 : list ty) : bool :=
+    match ts1, ts2 with
+    | nil, nil => true
+    | t1 :: ts1', t2 :: ts2' => andb (ty_compat t1 t2) (tys_compat ts1' ts2')
     | _, _ => false
     end.
 
   Lemma ty_compat_refl : forall t,
     ty_compat t t = true.
   Proof.
-    destruct t; unfold ty_compat;
-    match goal with
-    | [ |- (if ?X then _ else _) = _ ] => destruct X; congruence
-    end.
+    destruct t; unfold ty_compat; try apply eq_refl.
   Qed.
 
   Lemma ty_compat_sym : forall t1 t2,
     ty_compat t1 t2 = ty_compat t2 t1.
   Proof.
-    destruct t1, t2; try reflexivity;
-    match goal with
-    | [ |- ty_compat ?X ?Y = ty_compat ?Y ?X ] =>
-        destruct (ty_dec X Y) as [H1 | H1] eqn:EQ1;
-        destruct (ty_dec Y X) as [H2 | H2] eqn:EQ2;
-        try (inversion H1; reflexivity);
-        try (inversion H2; reflexivity);
-        try (unfold ty_compat; rewrite EQ1; rewrite EQ2; reflexivity)
-    end.
-    unfold ty_compat. repeat destruct ty_dec; try discriminate.
-    destruct (U.dec t t0); destruct (U.dec t0 t); congruence.
+    destruct t1, t2; unfold ty_compat; try rewrite eq_sym; try rewrite eq_refl; try reflexivity.
+    rewrite (@eq_sym U.t). reflexivity.
   Qed.
 
   Lemma ty_compat_simpl_eq : forall t1 t2,
@@ -193,8 +149,12 @@ Module Types' (U : UNIQUE).
     ty_compat t1 t2 = true ->
     t1 = t2.
   Proof.
-    intros; destruct H as [H | [H | H]]; destruct t2; try discriminate;
-    destruct t1; try discriminate; try reflexivity.
+    intros; destruct H as [H | [H | H]]; subst;
+    destruct t1; try reflexivity;
+    unfold ty_compat in H0;
+    match type of H0 with
+    | (if ?X then _ else _) = _ => destruct X
+    end; discriminate.
   Qed.
 
   Lemma ty_compat_arr : forall t1 t2 aty u,
@@ -202,8 +162,11 @@ Module Types' (U : UNIQUE).
     ty_compat t1 t2 = true ->
     t1 = t2.
   Proof.
-    intros; destruct t2; try discriminate; destruct t1; try discriminate;
-    unfold ty_compat in H0; destruct (ty_dec (ARRAY t1 t0) (ARRAY t2 t)); congruence.
+    intros. destruct t1, t2; try discriminate;
+    unfold ty_compat in H0;
+    match type of H0 with
+    | (if ?X then _ else _) = _ => destruct X
+    end; congruence.
   Qed.
 
   Lemma ty_compat_rec : forall fs1 fs2 u1 u2,
@@ -211,18 +174,18 @@ Module Types' (U : UNIQUE).
     u1 = u2.
   Proof.
     intros; unfold ty_compat in H;
-    destruct (ty_dec (RECORD fs1 u1) (RECORD fs2 u2));
-    destruct (U.dec u1 u2); congruence.
+    destruct (ty_eq (RECORD fs1 u1) (RECORD fs2 u2));
+    destruct (U.eq u1 u2); congruence.
   Qed.
 
   (* actual_ty might return another Name, but with the possibility of infinite cycles need to add a max depth *)
   Definition max_depth := 100.
 
-  Fixpoint actual_ty' (d : nat) (te : @Symbol.table ty) (t : ty) : option ty :=
+  Fixpoint actual_ty' (d : nat) (te : S.table ty) (t : ty) : option ty :=
     match d with
     | 0 => None
     | S d' => match t with
-        | NAME n => match Symbol.look te n with
+        | NAME n => match S.look te n with
             | None => None
             | Some t => actual_ty' d' te t
             end
@@ -232,7 +195,7 @@ Module Types' (U : UNIQUE).
 
   Definition actual_ty te t := actual_ty' max_depth te t.
 
-  Fixpoint actual_tys (te : @Symbol.table ty) (ts : list ty) : option (list ty) :=
+  Fixpoint actual_tys (te : S.table ty) (ts : list ty) : option (list ty) :=
     match ts with
     | nil => Some nil
     | t :: ts' => match actual_ty te t with
@@ -244,12 +207,11 @@ Module Types' (U : UNIQUE).
   Lemma actual_not_name' : forall te t n d,
     actual_ty' d te t <> Some (NAME n).
   Proof.
-    intros; destruct t;
-    try solve [destruct te, d; simpl; discriminate].
-    generalize dependent s; induction d; intros.
+    intros; destruct t; try solve [destruct d; simpl; discriminate].
+    generalize dependent t; induction d; intros.
     - discriminate.
-    - simpl. destruct (Symbol.look te s); try discriminate.
-      destruct t; try solve [destruct te, d; simpl; try discriminate].
+    - simpl. destruct (S.look te t); try discriminate.
+      destruct t0; try solve [destruct d; simpl; try discriminate].
       apply IHd.
   Qed.
 
@@ -284,4 +246,4 @@ Module Types' (U : UNIQUE).
 
 End Types'.
 
-Module Types := Types' Unique.
+Module Types := Types' Symbol Unique.
