util/DecEqFacts.v
@@ -1,0 +1,81 @@
+(*
+ * DecEqFacts.v
+ * Wolf Honore
+ *
+ * Some useful lemmas and functions related to decidable equality.
+ *)
+
+Require Import List.
+
+Section EQ_DEC.
+
+  Context {t : Type}.
+  Variable eq : forall (t1 t2 : t), {t1 = t2} + {t1 <> t2}.
+
+  Definition make_beq : t -> t -> bool :=
+    fun t1 t2 => if eq t1 t2 then true else false.
+
+  Section EQ_DEC_FACTS.
+
+    Lemma eq_refl {A} : forall t (b1 b2 : A),
+      (if eq t t then b1 else b2) = b1.
+    Proof.
+      intros; destruct (eq t0 t0); congruence.
+    Qed.
+
+    Lemma eq_sym {A} : forall t1 t2 (b1 b2 : A),
+      (if eq t1 t2 then b1 else b2) = (if eq t2 t1 then b1 else b2).
+    Proof.
+      intros; destruct (eq t1 t2).
+      - subst; symmetry; apply eq_refl.
+      - destruct (eq t2 t1); congruence.
+    Qed.
+
+    Lemma eq_true {A} : forall t1 t2 (b1 b2 : A),
+      t1 = t2 ->
+      (if eq t1 t2 then b1 else b2) = b1.
+    Proof.
+      intros; subst; apply eq_refl.
+    Qed.
+
+    Lemma eq_false {A} : forall t1 t2 (b1 b2 : A),
+      t1 <> t2 ->
+      (if eq t1 t2 then b1 else b2) = b2.
+    Proof.
+      intros; destruct (eq t1 t2); congruence.
+    Qed.
+
+  End EQ_DEC_FACTS.
+
+  (* Some of this is in the Coq standard library for versions > 8.4 *)
+  Section LIST_DEC_FACTS.
+
+    Fixpoint nodup (xs : list t) : bool :=
+      match xs with
+      | nil => true
+      | x :: xs' => if in_dec eq x xs' then false else nodup xs'
+      end.
+
+    Lemma nodup_sound : forall xs, nodup xs = true -> NoDup xs.
+    Proof.
+      induction xs.
+      - constructor.
+      - simpl. destruct (in_dec eq a xs).
+        + discriminate.
+        + constructor; auto.
+    Qed.
+
+    Lemma find_In : forall f (x : t) xs,
+      find f xs = Some x ->
+      In x xs.
+    Proof.
+      intros. induction xs.
+      - discriminate.
+      - inversion H. destruct (f a).
+        + inversion H1; simpl; auto.
+        + simpl; auto.
+    Qed.
+
+  End LIST_DEC_FACTS.
+
+End EQ_DEC.
